

Vertical motion equation

$$\left(\Psi_{j,k}^{(m)}(t)\right)_{L,1} = (X_{j,k})_{L,1} e^{\lambda t}$$

$$j = 2, 3, \dots, J; k = 1, 2, \dots, K + 1; L = (J - 1)(K + 1)$$

$$\nabla^2 w + \frac{f_0^2}{N^2} \frac{\partial^2 w}{\partial Z^2} = \frac{f_0}{N^2} (F_1 + F_2 + F_3)$$

Meridional (background) temperature advection: $F_1 = 2 \frac{\partial \bar{u}}{\partial z} \frac{\partial}{\partial x} \nabla^2 \psi'$

Vertical differential meridional (background) vorticity advection: $F_2 = -2 \frac{\partial^2 \bar{u}}{\partial y^2} \frac{\partial^2 \psi'}{\partial z \partial x}$

Vertical differential meridional planetary vorticity advection: $F_3 = \beta \frac{\partial^2 \psi'}{\partial z \partial x}$

The boundary conditions for w :

$$\begin{aligned} x: w(x = 0, y, Z, t) &= w(x = L_x, y, Z, t); \\ Z: w(x, y, Z = 0, t) &= w(x, y, Z = H, t) = 0; \\ y: &\text{no condition (i.e., part of the solution)} \end{aligned}$$

Numerical scheme for solving for vertical motion equation

$$\nabla^2 w + \frac{f_0^2}{N^2} \frac{\partial^2 w}{\partial Z^2} = \frac{f_0^2}{N^2} (F_1 + F_2 + F_3)$$

The boundary conditions for w :

x : $w(x = 0, y, Z, t) = w(x = L_x, y, Z, t)$;
 Z : $w(x, y, Z = 0, t) = w(x, y, Z = H, t) = 0$;
 y : *no condition (i.e., part of the solution)*

Symbolically, we can write the vertical motion equation at 2D grids for **each zonal wave m** as

$$G_{LW,LW}(w_{j,k})_{LW,1} = \frac{f_0}{N^2} \{ (F1_{j,k})_{LW,1} + (F2_{j,k})_{LW,1} + (F3_{j,k})_{LW,1} \}$$

$$j = 1, 2, 3, \dots, J, \textcolor{red}{J+1}; k = 2, 3, \dots, \textcolor{red}{K}; LW = (\textcolor{red}{J+1})(\textcolor{red}{K-1})$$

From grid-vector to column-vector:

$$l(j, k) = j + (k - 2)(J + 1)$$

From column-vector to grid-vector:

$$k(l) = \text{int} \left\{ \frac{l - 1}{(J + 1)} \right\} + 2;$$

$$j(l) = l - (k - 2)(J + 1)$$

Numerical scheme for calculating $\nabla^2 w + \frac{f_0^2}{N^2} \frac{\partial^2 w}{\partial Z^2}$

$$w_{i,j,k} = \text{Re}\{W^{(m)}(y_j, Z_k) e^{\sqrt{-1} \frac{2\pi m}{L_x} x_i}\}$$

$$(EW)_{j,k} = (\nabla^2 w)_{j,k} + \frac{f_0^2}{N^2} \left(\frac{\partial^2 w}{\partial Z^2} \right)_{j,k}$$

$$j = 1, 2, 3, \dots, J, J+1; k = 2, 3, \dots, K; LW = (J+1)(K-1)$$

for $1 < j < J$ and all k :

$$(EW)_{j,k} = -\left(\frac{2\pi m}{L_x}\right)^2 W_{j,k}^{(m)} + \frac{W_{j+1,k}^{(m)} - 2W_{j,k}^{(m)} + W_{j-1,k}^{(m)}}{\Delta y^2} + \frac{f_0^2}{N^2} \frac{W_{j,k+1}^{(m)} - 2W_{j,k}^{(m)} + W_{j,k-1}^{(m)}}{\Delta Z^2}$$

for $j = 1$ and all k :

$$(EW)_{1,k} = -\left(\frac{2\pi m}{L_x}\right)^2 W_{1,k}^{(m)} + \frac{W_{3,k}^{(m)} - 2W_{2,k}^{(m)} + W_{1,k}^{(m)}}{\Delta y^2} + \frac{f_0^2}{N^2} \frac{W_{1,k+1}^{(m)} - 2W_{1,k}^{(m)} + W_{1,k-1}^{(m)}}{\Delta Z^2}$$

for $j = J+1$ and all k :

$$\begin{aligned} & (EW)_{J+1,k} \\ &= -\left(\frac{2\pi m}{L_x}\right)^2 W_{J+1,k}^{(m)} + \frac{W_{J+1,k}^{(m)} - 2W_{J,k}^{(m)} + W_{J-1,k}^{(m)}}{\Delta y^2} + \frac{f_0^2}{N^2} \frac{W_{J+1,k+1}^{(m)} - 2W_{J+1,k}^{(m)} + W_{J+1,k-1}^{(m)}}{\Delta Z^2} \end{aligned}$$

Algorithm for obtaining matrix $G_{LW,LW}$ numerically

$$LW = (J + 1) \times (K - 1)$$

Step 1. Define a column vector of length L , \vec{x}_n , in which all elements are zero except the one at the n^{th} column, which equals 1, $1 \leq n \leq LW$.

$$\vec{x}_n = \begin{pmatrix} x_1 = 0 \\ \vdots \\ x_{n-1} = 0 \\ x_n = 1 \\ x_{n+1} = 0 \\ \vdots \\ x_{LW} = 0 \end{pmatrix}_{LW,1}$$

Step 2. Applying the conversion from a column-vector to a grid vector, $k(lw)$, and $j(lw)$, convert the column vector \vec{x}_n to its grid – vector counterpart, denoted as $(x_{j,k}^{(n)})$.

Step 3. Repeat Step 1 thorough Step 2 from $n = 1, n = 2, \dots, n = LW$, we will obtain all LW columns of $G_{LW,LW}$.

Algorithm for obtaining F1, F2, and F3

$$LW = (J + 1) \times (K - 1)$$

$$G_{LW,LW}(w_{j,k})_{LW,1} = \frac{f_0}{N^2} \{ (F1_{j,k})_{LW,1} + (F2_{j,k})_{LW,1} + (F3_{j,k})_{LW,1} \}$$

$$(w_{j,k})_{LW,1} = \frac{f_0}{N^2} (G_{LW,LW})^{-1} \{ (F1_{j,k})_{LW,1} + (F2_{j,k})_{LW,1} + (F3_{j,k})_{LW,1} \}$$

$$j = 1, 2, 3, \dots, J, J + 1; k = 2, 3, \dots, K; LW = (J + 1)(K - 1)$$

$$\text{Meridional (background) temperature advection: } F_1 = 2 \frac{\partial \bar{u}}{\partial z} \frac{\partial}{\partial x} \nabla^2 \psi'$$

$$\text{Vertical differential meridional (background) vorticity advection: } F_2 = -2 \frac{\partial^2 \bar{u}}{\partial y^2} \frac{\partial^2 \psi'}{\partial z \partial x}$$

$$\text{Vertical differential meridional planetary vorticity advection: } F_3 = \beta \frac{\partial^2 \psi'}{\partial z \partial x}$$

Algorithm for obtaining F1, F2, and F3

$$LW = (J + 1) \times (K - 1)$$

$$F_3 = \beta \frac{\partial^2 \psi'}{\partial z \partial x}$$

$$j = 1, 2, 3, \dots, J, J + 1; k = 2, 3, \dots, K; LW = (J + 1)(K - 1)$$

for $1 < j < J + 1$ *and all* k :

$$(F3_{j,k}) = \sqrt{-1} \frac{2\pi m}{L_x} \beta \left(\frac{\Psi_{j,k+1}^{(m)} - \Psi_{j,k-1}^{(m)}}{2\Delta z} \right)$$

for $j = 1$ *and all* k :

$$(F3_{j,k}) = 0$$

for $j = J + 1$ *and all* k :

$$(F3_{j,k}) = 0$$

Algorithm for obtaining F1, F2, and F3

$$LW = (J + 1) \times (K - 1)$$

$$F_2 = -2 \frac{\partial^2 \bar{u}}{\partial y^2} \frac{\partial^2 \psi'}{\partial z \partial x}$$

$$j = 1, 2, 3, \dots, J, J + 1; k = 2, 3, \dots, K; LW = (J + 1)(K - 1)$$

for $1 < j < J + 1$ and all k :

$$(F2_{j,k}) = -2\sqrt{-1} \frac{2\pi m}{L_x} \frac{(\bar{u}_{j+1,k} - 2\bar{u}_{j,k} + \bar{u}_{j-1,k})}{\Delta y^2} \left(\frac{\Psi_{j,k+1}^{(m)} - \Psi_{j,k-1}^{(m)}}{2\Delta z} \right)$$

for $j = 1$ and all k :

$$(F2_{j,k}) = 0$$

for $j = J + 1$ and all k :

$$(F2_{j,k}) = 0$$

Algorithm for obtaining F1, F2, and F3

$$F_1 = 2 \frac{\partial \bar{u}}{\partial z} \frac{\partial}{\partial x} \nabla^2 \psi'$$

$$j = 1, 2, 3, \dots, J, \textcolor{red}{J+1}; k = 2, 3, \dots, \textcolor{red}{K};$$

$$LW = (J+1) \times (K-1)$$

for $2 < j < J$ and all k :

$$(F1_{j,k}) = 2\sqrt{-1} \frac{2\pi m}{L_x} \frac{(\bar{u}_{j,k+1} - \bar{u}_{j,k-1})}{2\Delta z} \left(- \left(\frac{2\pi m}{L_x} \right)^2 \Psi_{j,k}^{(m)} + \frac{\Psi_{j+1,k}^{(m)} - 2\Psi_{j,k}^{(m)} + \Psi_{j-1,k}^{(m)}}{\Delta y^2} \right)$$

$$\textit{for } j = 1: (F1_{j,k}) = 2\sqrt{-1} \frac{2\pi m}{L_x} \frac{(\bar{u}_{j,k+1} - \bar{u}_{j,k-1})}{2\Delta z} \left(\frac{\Psi_{3,k}^{(m)} - 2\Psi_{2,k}^{(m)} + 0}{\Delta y^2} \right)$$

$$\textit{for } j = 2: (F1_{j,k}) = 2\sqrt{-1} \frac{2\pi m}{L_x} \frac{(\bar{u}_{j,k+1} - \bar{u}_{j,k-1})}{2\Delta z} \left(- \left(\frac{2\pi m}{L_x} \right)^2 \Psi_{j,k}^{(m)} + \frac{\Psi_{3,k}^{(m)} - 2\Psi_{2,k}^{(m)} + 0}{\Delta y^2} \right)$$

$$\textit{for } j = J: (F1_{j,k}) = 2\sqrt{-1} \frac{2\pi m}{L_x} \frac{(\bar{u}_{j,k+1} - \bar{u}_{j,k-1})}{2\Delta z} \left(\frac{0 - 2\Psi_{J,k}^{(m)} + \Psi_{J-2,k}^{(m)}}{\Delta y^2} \right)$$

$$\textit{for } j = J+1: (F1_{j,k}) = 2\sqrt{-1} \frac{2\pi m}{L_x} \frac{(\bar{u}_{j,k+1} - \bar{u}_{j,k-1})}{2\Delta z} \left(\frac{0 - 2\Psi_{j-1,k}^{(m)} + \Psi_{j-2,k}^{(m)}}{\Delta y^2} \right)$$

3D vertical motion field

$$w_{i,j,k}(t = 0) = \text{Re} \left\{ \left(W_{j,k}^{(n)} \right)_{LW,1} e^{\sqrt{-1} \frac{2\pi m}{L_x} x_i} \right\}$$

$$[j, k] = lW2jk(l), l = 1, 2 \dots LW$$

$$\begin{aligned} & \text{for } j = 1, 3, \dots, J + 1; k = 2, \dots, K \\ & w_{i,j,k}(t = 0) = \text{Re} \left\{ \left(W_l^{(n)} \right)_{LW,1} e^{\sqrt{-1} \frac{2\pi m}{L_x} x_i} \right\} \\ & x_i = (i - 1)\Delta x, i = 1, 2, \dots, 360; \Delta x = Lx/360 \end{aligned}$$

$$\begin{aligned} & \text{for } k = 1 \text{ and } k = K + 1; j = 1, 2, \dots, J + 1; i = 1, 2, \dots, 360 \\ & w_{i,j,k}(t = 0) = 0 \end{aligned}$$